proof/auditor_proof/rpc.v
@@ -1,2 +1,269 @@
+From New.generatedproof.github_com.sanjit_bhat.pav Require Import auditor server.
+From New.proof.github_com.sanjit_bhat.pav Require Import prelude.
+
+From New.proof.github_com.sanjit_bhat.pav Require Import
+  advrpc cryptoffi hashchain ktcore merkle.
+
+From New.proof.github_com.sanjit_bhat.pav.server_proof Require Import
+  serde server rpc.
+
 Module auditor.
+Import serde.server server.server rpc.server.
+
+Module state.
+Record t :=
+  mk {
+    start_ep: w64;
+    links: list $ list w8;
+  }.
+End state.
+
+(* cfg is the static state we know about this party, if good. *)
+Module cfg.
+Record t :=
+  mk {
+    serv_sig_pk: list w8;
+    adtr_sig_pk: list w8;
+    sigpredγ: ktcore.sigpred_cfg.t;
+    vrf_pk: list w8;
+    serv_good: option $ server.cfg.t;
+  }.
+End cfg.
+
+Module epoch.
+Record t :=
+  mk' {
+    link: list w8;
+  }.
+
+Section proof.
+Context `{hG: heapGS Σ, !ffi_semantics _ _, !globalsGS Σ} {go_ctx : GoContext}.
+
+Definition own ptr obj ep γ : iProp Σ :=
+  ∃ sl_link sl_servSig servSig sl_adtrSig adtrSig,
+  "#Hstr_epoch" ∷ ptr ↦□ (auditor.epoch.mk sl_link sl_servSig sl_adtrSig) ∗
+  "#Hsl_link" ∷ sl_link ↦*□ obj.(link) ∗
+  "#Hsl_servSig" ∷ sl_servSig ↦*□ servSig ∗
+  "#His_servSig" ∷ ktcore.wish_LinkSig γ.(cfg.serv_sig_pk) ep obj.(link) servSig ∗
+  "#Hsl_adtrSig" ∷ sl_adtrSig ↦*□ adtrSig ∗
+  "#His_adtrSig" ∷ ktcore.wish_LinkSig γ.(cfg.adtr_sig_pk) ep obj.(link) adtrSig.
+
+End proof.
+End epoch.
+
+Module history.
+Record t :=
+  mk' {
+    digs: list $ list w8;
+    cut: option $ list w8;
+  }.
+
+Section proof.
+Context `{hG: heapGS Σ, !ffi_semantics _ _, !globalsGS Σ} {go_ctx : GoContext}.
+Context `{!pavG Σ}.
+
+Definition own ptr obj γ σ q : iProp Σ :=
+  ∃ sl_lastDig lastDig sl_epochs sl0_epochs (last_ep : w64),
+  "Hstr_history" ∷ ptr ↦{#q} (auditor.history.mk sl_lastDig σ.(state.start_ep) sl_epochs) ∗
+  "#Hsl_lastDig" ∷ sl_lastDig ↦*□ lastDig ∗
+  "%Heq_lastDig" ∷ ⌜last obj.(digs) = Some lastDig⌝ ∗
+  "Hsl_epochs" ∷ sl_epochs ↦*{#q} sl0_epochs ∗
+  "Hcap_epochs" ∷ own_slice_cap loc sl_epochs (DfracOwn q) ∗
+  "#Hepochs" ∷ ([∗ list] idx ↦ p;o ∈ sl0_epochs;σ.(state.links),
+    epoch.own p (epoch.mk' o) (uint.nat σ.(state.start_ep) + idx) γ) ∗
+  "%Hsome_links" ∷ ⌜length σ.(state.links) > 0⌝ ∗
+  "%Hinb_ep" ∷ ⌜uint.Z σ.(state.start_ep) + length σ.(state.links) - 1 =
+    uint.Z last_ep⌝.
+
+Definition own_gs γ σ q : iProp Σ :=
+  "#Hgs_start_ep" ∷ ghost_var γ.(cfg.sigpredγ).(ktcore.sigpred_cfg.start_ep)
+    (□) σ.(state.start_ep) ∗
+  (* 1/2 own in fupd inv. *)
+  "Hgs_links" ∷ mono_list_auth_own γ.(cfg.sigpredγ).(ktcore.sigpred_cfg.links)
+    (q/2) σ.(state.links).
+
+Definition align_serv obj σ servγ : iProp Σ :=
+  ∃ hist,
+  "#His_hist" ∷ mono_list_lb_own servγ.(server.cfg.histγ) hist ∗
+  "%Heq_ep" ∷ ⌜length hist = (uint.nat σ.(state.start_ep) + length σ.(state.links))%nat⌝ ∗
+  "%Heq_digs" ∷ ⌜obj.(digs) = hist.*1⌝ ∗
+  "%Heq_cut" ∷ ⌜obj.(cut) = None⌝.
+
+End proof.
+End history.
+
+Section proof.
+Context `{hG: heapGS Σ, !ffi_semantics _ _, !globalsGS Σ} {go_ctx : GoContext}.
+Context `{!pavG Σ}.
+
+Definition wish_getNextLink sig_pk hist σ proof (ep : w64) dig link : iProp Σ :=
+  ∃ prevDig,
+  "%Heq_ep" ∷ ⌜uint.Z ep = (uint.Z σ.(state.start_ep) + length σ.(state.links))%Z⌝ ∗
+  "%Heq_prevDig" ∷ ⌜last hist.(history.digs) = Some prevDig⌝ ∗
+  "#His_upd" ∷ ktcore.wish_ListUpdate prevDig
+    proof.(ktcore.AuditProof.Updates) dig ∗
+  "#His_link" ∷ hashchain.is_chain (hist.(history.digs) ++ [dig])
+    hist.(history.cut) link (S $ uint.nat ep) ∗
+  "#His_sig" ∷ ktcore.wish_LinkSig sig_pk ep link
+    proof.(ktcore.AuditProof.LinkSig).
+
+Lemma wish_getNextLink_det sig_pk hist σ proof ep0 dig0 link0 ep1 dig1 link1 :
+  wish_getNextLink sig_pk hist σ proof ep0 dig0 link0 -∗
+  wish_getNextLink sig_pk hist σ proof ep1 dig1 link1 -∗
+  ⌜ep0 = ep1 ∧ dig0 = dig1 ∧ link0 = link1⌝.
+Proof.
+  iNamedSuffix 1 "0".
+  iNamedSuffix 1 "1".
+  simplify_eq/=.
+  iDestruct (ktcore.wish_ListUpdate_det with "His_upd0 His_upd1") as %->.
+  iDestruct (hashchain.is_chain_det with "His_link0 His_link1") as %->.
+  iPureIntro. repeat split. word.
+Qed.
+
+Lemma wp_CallAudit s good (prevEpoch : w64) :
+  {{{
+    is_pkg_init server ∗
+    "#His_serv" ∷ is_Server_rpc s good ∗
+    "#His_args" ∷ match good with None => True | Some γ =>
+      ∃ (entry : list w8 * keys_ty),
+      "#Hidx_ep" ∷ mono_list_idx_own γ.(cfg.histγ) (uint.nat prevEpoch) entry end
+  }}}
+  @! server.CallAudit #s #prevEpoch
+  {{{
+    sl_proofs err, RET (#sl_proofs, #(ktcore.blame_to_u64 err));
+    "%Hblame" ∷ ⌜ktcore.BlameSpec err {[ktcore.BlameServFull:=option_bool good]}⌝ ∗
+    "Herr" ∷ (if decide (err ≠ ∅) then True else
+      ∃ proofs,
+      "#Hsl_proofs" ∷ ktcore.AuditProofSlice1D.own sl_proofs proofs (□) ∗
+
+      "Hgood" ∷ match good with None => True | Some γ =>
+        "%Hnoof_eps" ∷ ⌜let numEps := (uint.Z prevEpoch + length proofs + 1)%Z in
+          numEps = sint.nat (W64 $ numEps)⌝ ∗
+        (* writing determ trans per epoch makes postcond easier to use
+        than one trans across all epochs. epochs are indep. *)
+        "Hproofs" ∷ ([∗ list] idx ↦ proof ∈ proofs,
+          ∀ adtr_hist adtrσ,
+          history.align_serv adtr_hist adtrσ γ -∗
+          ⌜uint.Z adtrσ.(state.start_ep) + length adtrσ.(state.links) - 1 =
+            (uint.Z prevEpoch + idx)%Z⌝ -∗
+
+          ∃ ep dig link,
+          let adtr_hist' := set history.digs (.++ [dig]) adtr_hist in
+          let adtrσ' := set state.links (.++ [link]) adtrσ in
+          "#Hwish_getNextLink" ∷ wish_getNextLink γ.(cfg.sig_pk)
+            adtr_hist adtrσ proof ep dig link ∗
+          "#Halign_next" ∷ history.align_serv adtr_hist' adtrσ' γ) end)
+  }}}.
+Proof.
+  wp_start as "@". wp_auto.
+  wp_apply wp_alloc as "* Ha".
+  wp_apply (AuditArg.wp_enc (AuditArg.mk' _) with "[$Ha]") as "* (Hsl_b&_&_&%Hwish)".
+  { iDestruct own_slice_nil as "$".
+    iDestruct own_slice_cap_nil as "$". }
+  simpl in *.
+  wp_apply wp_alloc as "* Hreply".
+  wp_apply (wp_Audit_cli_call (Q_read (uint.nat prevEpoch))
+    with "[$Hsl_b $Hreply]") as "* @".
+  { iFrame "#". case_match; try done.
+    iModIntro.
+    iNamed "His_args".
+    by iApply op_read. }
+  wp_if_destruct.
+  { rewrite ktcore.rw_BlameUnknown.
+    iApply "HΦ".
+    iSplit; [|by case_decide].
+    iPureIntro. apply ktcore.blame_unknown. }
+  iNamed "Herr_net".
+  iPersist "Hsl_reply".
+  wp_apply (AuditReply.wp_dec with "[$Hsl_reply]") as "* Hgenie".
+  wp_if_destruct.
+  { rewrite ktcore.rw_BlameServFull.
+    iApply "HΦ".
+    iSplit; [|by case_decide].
+    iApply ktcore.blame_one.
+    iIntros (?).
+    case_match; try done.
+    iNamed "Hgood".
+    iApply "Hgenie".
+    naive_solver. }
+  iDestruct "Hgenie" as (??) "(#Hreply&_&%His_dec)".
+  destruct obj. iNamed "Hreply".
+  wp_auto. simpl.
+  wp_if_destruct.
+  { rewrite ktcore.rw_BlameServFull.
+    iApply "HΦ".
+    iSplit; try done.
+    iApply ktcore.blame_one.
+    iIntros (?).
+    case_match; try done.
+    iNamed "Hgood".
+    opose proof (AuditReply.wish_det _ _ _ _ His_dec His_reply) as [? _].
+    simplify_eq/=.
+    iDestruct "Hgood" as "[@|@]".
+    - iApply "Hgenie". naive_solver.
+    - opose proof (AuditArg.wish_det _ _ _ _ Hwish Hdec) as [? _].
+      simplify_eq/=.
+      iDestruct "HQ" as "[#Hnew_hist %]".
+      iDestruct "Herr" as %?.
+      lia. }
+
+  rewrite /ktcore.BlameNone ktcore.rw_BlameNone.
+  iApply "HΦ".
+  iSplit.
+  { iPureIntro. apply ktcore.blame_none. }
+  case_decide; try done.
+  iFrame "#".
+  case_match; try done.
+  iNamed "Hgood".
+  opose proof (AuditReply.wish_det _ _ _ _ His_dec His_reply) as [? _].
+  simplify_eq/=.
+  iDestruct "Hgood" as "[@|@]"; try done.
+  opose proof (AuditArg.wish_det _ _ _ _ Hwish Hdec) as [? _].
+  simplify_eq/=.
+  iDestruct "HQ" as "[#Hnew_hist %]".
+  iNamed "Herr".
+
+  iSplit; [word|].
+  iClear "His_args".
+  iApply big_sepL_intro.
+  iModIntro. iIntros (?? Hlook_proofs ??) "@ %".
+  rewrite /wish_getNextLink /history.align_serv.
+  destruct adtr_hist, σ. simplify_eq/=.
+  iDestruct (big_sepL_lookup with "His_upds") as "{His_upds} @"; [done|].
+  iDestruct (big_sepL_lookup with "His_sigs") as "{His_sigs} @"; [done|].
+  apply lookup_lt_Some in Hlook_proofs.
+  iDestruct (mono_list_lb_valid with "Hnew_hist His_hist") as %[[? Hpref]|[new_hist ?]].
+  { apply (f_equal length) in Hpref.
+    autorewrite with len in *. word. }
+  simplify_eq/=.
+  autorewrite with len in *.
+  pose proof Hlook1 as Ht.
+  apply list_lookup_fmap_Some_1 in Ht as (new_ep&?&Hlook_new).
+  iDestruct (mono_list_lb_own_le (hist ++ [new_ep]) with "Hnew_hist")
+    as "{Hnew_hist His_hist} Hlb".
+  { apply prefix_snoc.
+    { by apply prefix_app_r. }
+    rewrite -Hlook_new. f_equal. word. }
+
+  iFrame "#".
+  autorewrite with len.
+  repeat iSplit; try done; try iPureIntro.
+  - word.
+  - apply list_lookup_fmap_Some_1 in Hlook0 as (?&?&Ht).
+    rewrite lookup_app_l in Ht; [|word].
+    replace (_ + _)%nat with (pred $ length hist) in Ht by word.
+    rewrite -last_lookup in Ht.
+    rewrite fmap_last Ht.
+    naive_solver.
+  - iExactEq "His_link". rewrite /named. f_equal; [|word].
+    erewrite take_S_r.
+    + f_equal.
+      rewrite fmap_app take_app_length'; [done|].
+      len.
+    + rewrite -Hlook1. f_equal. word.
+  - word.
+  - rewrite fmap_app. naive_solver.
+Qed.
+
+End proof.
 End auditor.
